Nerodia/Data/TypeExpr.lean
@@ -7,25 +7,10 @@ module
 
 namespace Nerodia
 
-/-- An identifier of a Python type constant (e.g., {lean}`"str"`). -/
-public structure TypeConst where
-  ofString ::
-    protected toString : String
-    deriving Nonempty, DecidableEq
-
-public instance : ToString TypeConst := ⟨TypeConst.toString⟩
-
 /-- A Python type expression. -/
 public structure TypeExpr where
   ofString ::
     protected toString : String
     deriving Nonempty, DecidableEq
 
-namespace TypeExpr
-
 public instance : ToString TypeExpr := ⟨TypeExpr.toString⟩
-
-@[inline, irreducible, expose] public def ofTypeConst (n : TypeConst) : TypeExpr :=
-  ⟨n.toString⟩
-
-public instance : Coe TypeConst TypeExpr := ⟨ofTypeConst⟩
